<?xml version="1.0" encoding="UTF-8"?>
<!--

    #-=-=-=-=-=-=-=-=-=-=-=-=-=-=-=-=-=-=-=-=-=-=-=-=-=-=-=-=-=-=-=-=-=-=-=-=-=#
      This file is part of the Smart Developer Hub Project:
        http://smartdeveloperhub.github.io/

      Center for Open Middleware
        http://www.centeropenmiddleware.com/
    #-=-=-=-=-=-=-=-=-=-=-=-=-=-=-=-=-=-=-=-=-=-=-=-=-=-=-=-=-=-=-=-=-=-=-=-=-=#
      Copyright (C) 2015 Center for Open Middleware.
    #-=-=-=-=-=-=-=-=-=-=-=-=-=-=-=-=-=-=-=-=-=-=-=-=-=-=-=-=-=-=-=-=-=-=-=-=-=#
      Licensed under the Apache License, Version 2.0 (the "License");
      you may not use this file except in compliance with the License.
      You may obtain a copy of the License at

                http://www.apache.org/licenses/LICENSE-2.0

      Unless required by applicable law or agreed to in writing, software
      distributed under the License is distributed on an "AS IS" BASIS,
      WITHOUT WARRANTIES OR CONDITIONS OF ANY KIND, either express or implied.
      See the License for the specific language governing permissions and
      limitations under the License.
    #-=-=-=-=-=-=-=-=-=-=-=-=-=-=-=-=-=-=-=-=-=-=-=-=-=-=-=-=-=-=-=-=-=-=-=-=-=#
      Artifact    : org.sdh.vocabulary:sdh-vocabulary:1.0.0-SNAPSHOT
      Bundle      : sdh-vocabulary-1.0.0-SNAPSHOT.jar
    #-=-=-=-=-=-=-=-=-=-=-=-=-=-=-=-=-=-=-=-=-=-=-=-=-=-=-=-=-=-=-=-=-=-=-=-=-=#

-->
<rdf:RDF xmlns:rdf="http://www.w3.org/1999/02/22-rdf-syntax-ns#"
	xmlns:rdfs="http://www.w3.org/2000/01/rdf-schema#" xmlns:owl="http://www.w3.org/2002/07/owl#"
	xmlns:dcterms="http://purl.org/dc/terms/" xmlns:rddl="http://www.rddl.org/">
	<owl:Ontology rdf:about="http://open-services.net/ns/auto#">
		<dcterms:title>The OSLC Automation Vocabulary</dcterms:title>
		<dcterms:description>
			All vocabulary
			URIs defined in the OSLC Automation namespace.
		</dcterms:description>
		<rdfs:label>Automation</rdfs:label>
		<rdfs:seeAlso rdf:resource="http://open-services.net/wiki/automation" />
		<rdfs:seeAlso
			rdf:resource="http://open-services.net/wiki/automation/OSLC-Automation-Specification-Version-2.1/" />
		<rdfs:seeAlso
			rdf:resource="http://open-services.net/wiki/automation/OSLC-Automation-Specification-Version-2.0/" />
		<rdfs:seeAlso rdf:resource="http://open-services.net/ns/auto/auto.rdf" />
		<rdfs:seeAlso>
			<rdf:Description rdf:about="http://open-services.net/ns/auto/auto.rdf">
				<rddl:nature rdf:resource="http://www.w3.org/2000/01/rdf-schema#" />
			</rdf:Description>
		</rdfs:seeAlso>
		<dcterms:source rdf:resource="http://open-services.net/ns/auto/auto.rdf" />
	</owl:Ontology>

	<rdfs:Class rdf:about="http://open-services.net/ns/auto#AutomationPlan">
		<rdfs:isDefinedBy rdf:resource="http://open-services.net/ns/auto#" />
		<rdfs:label>AutomationPlan</rdfs:label>
		<rdfs:comment>The Automation Plan resource</rdfs:comment>
		<rdfs:seeAlso
			rdf:resource="http://open-services.net/wiki/automation/OSLC-Automation-Specification-Version-2.0/#Resource_AutomationPlan" />
	</rdfs:Class>

	<rdfs:Class rdf:about="http://open-services.net/ns/auto#AutomationRequest">
		<rdfs:isDefinedBy rdf:resource="http://open-services.net/ns/auto#" />
		<rdfs:label>AutomationRequest</rdfs:label>
		<rdfs:comment>The Automation Request resource</rdfs:comment>
		<rdfs:seeAlso
			rdf:resource="http://open-services.net/wiki/automation/OSLC-Automation-Specification-Version-2.0/#Resource_AutomationRequest" />
	</rdfs:Class>

	<rdfs:Class rdf:about="http://open-services.net/ns/auto#AutomationResult">
		<rdfs:isDefinedBy rdf:resource="http://open-services.net/ns/auto#" />
		<rdfs:label>AutomationResult</rdfs:label>
		<rdfs:comment>The Automation Result resource</rdfs:comment>
		<rdfs:seeAlso
			rdf:resource="http://open-services.net/wiki/automation/OSLC-Automation-Specification-Version-2.0/#Resource_AutomationResult" />
	</rdfs:Class>

	<rdfs:Class rdf:about="http://open-services.net/ns/auto#ParameterInstance">
		<rdfs:isDefinedBy rdf:resource="http://open-services.net/ns/auto#" />
		<rdfs:label>ParameterInstance</rdfs:label>
		<rdfs:comment>The Automation Parameter Instance resource
		</rdfs:comment>
		<rdfs:seeAlso
			rdf:resource="http://open-services.net/wiki/automation/OSLC-Automation-Specification-Version-2.0/#Resource_ParameterInstance" />
	</rdfs:Class>



	<rdf:Property rdf:about="http://open-services.net/ns/auto#parameterDefinition">
		<rdfs:isDefinedBy rdf:resource="http://open-services.net/ns/auto#" />
		<rdfs:label>parameterDefinition</rdfs:label>
		<rdfs:comment>The definition of a parameter for this Automation Plan.
			parameterDefinitions are either a local (inline) or referenced
			resource and use the attributes (the range) of the oslc:Property
			resource with one exception. When used in the context of an
			oslc_auto:parameterDefinition, the cardinality of
			`oslc:propertyDefinition` becomes zero-or-one instead of exactly-one.
			Automation consumers creating Automation Requests *MUST* use the
			`oslc:occurs` attribute of the parameterDefinition, if present, to
			determine if a given parameter is required when creating the
			Automation Request. If the `oslc:occurs` attribute indicates the
			parameter is required (exactly-one or one-or-more), the service
			provider must guarantee the named parameter will be present in the
			Automation Result either as an `oslc_auto:inputParameter` when
			unmodified during execution, or as an `oslc_auto:outputParameter`
			when modified during execution.
		</rdfs:comment>
		<rdfs:range rdf:resource="http://open-services.net/ns/auto#AutomationPlan" />
		<rdfs:seeAlso
			rdf:resource="http://open-services.net/wiki/automation/OSLC-Automation-Specification-Version-2.0/#Resource_AutomationPlan" />
	</rdf:Property>

	<rdf:Property rdf:about="http://open-services.net/ns/auto#inputParameter">
		<rdfs:isDefinedBy rdf:resource="http://open-services.net/ns/auto#" />
		<rdfs:label>inputParameter</rdfs:label>
		<rdfs:comment>Parameters provided when Automation Requests are
			created. These include parameters provided by the creator of the
			Automation Request (whether by delegated UI or HTTP POST) and *MAY*
			include additional parameters added by the service provider during
			Automation Request creation. See the definition of the
			`oslc_auto:parameterDefinition` attribute of the Automation Plan for
			additional guidance on determining which parameters are required.
			Creators of Automation Requests *MAY* provide parameters beyond those
			defined in the Automation Plan without guarantee the service provider
			will recognize or honor them. It is expected that this attribute is
			write-able on Automation Request creation and read-only thereafter.
		</rdfs:comment>
		<rdfs:range rdf:resource="http://open-services.net/ns/auto#AutomationRequest" />
		<rdfs:range rdf:resource="http://open-services.net/ns/auto#AutomationResult" />
		<rdfs:seeAlso
			rdf:resource="http://open-services.net/wiki/automation/OSLC-Automation-Specification-Version-2.0/#Resource_AutomationRequest" />
		<rdfs:seeAlso
			rdf:resource="http://open-services.net/wiki/automation/OSLC-Automation-Specification-Version-2.0/#Resource_AutomationResult" />
	</rdf:Property>

	<rdf:Property rdf:about="http://open-services.net/ns/auto#state">
		<rdfs:isDefinedBy rdf:resource="http://open-services.net/ns/auto#" />
		<rdfs:label>state</rdfs:label>
		<rdfs:comment>Used to indicate the state of the automation request or
			result based on values defined in the automation specification and,
			optionally, by the service provider. Most often a read-only property.
			It is expected that this will be a resource reference to a definition
			of a valid automation request or result state on the service
			provider.
		</rdfs:comment>
		<rdfs:range rdf:resource="http://open-services.net/ns/auto#AutomationRequest" />
		<rdfs:range rdf:resource="http://open-services.net/ns/auto#AutomationResult" />
		<rdfs:seeAlso
			rdf:resource="http://open-services.net/wiki/automation/OSLC-Automation-Specification-Version-2.0/#Resource_AutomationRequest" />
		<rdfs:seeAlso
			rdf:resource="http://open-services.net/wiki/automation/OSLC-Automation-Specification-Version-2.0/#Resource_AutomationResult" />
	</rdf:Property>

	<rdf:Property rdf:about="http://open-services.net/ns/auto#desiredState">
		<rdfs:isDefinedBy rdf:resource="http://open-services.net/ns/auto#" />
		<rdfs:label>desiredState</rdfs:label>
		<rdfs:comment>The intended (domain- or provider-dependant) value of a resource's (domain-dependant) "state" property after some (future, present or past) process, transition or change. It is expected that this will be a resource reference to a definition of a valid state on the service provider. For example, in the OSLC Automation domain this is used to indicate the desired state of the Automation Request based on values defined in the OSLC Automation specification and, optionally, by the service provider.
		</rdfs:comment>
		<rdfs:range rdf:resource="http://open-services.net/ns/auto#AutomationRequest" />
		<rdfs:range rdf:resource="http://open-services.net/ns/auto#AutomationResult" />
		<rdfs:seeAlso
			rdf:resource="http://open-services.net/wiki/automation/OSLC-Automation-Specification-Version-2.0/#Resource_AutomationRequest" />
		<rdfs:seeAlso
			rdf:resource="http://open-services.net/wiki/automation/OSLC-Automation-Specification-Version-2.0/#Resource_AutomationResult" />
	</rdf:Property>

	<rdf:Property rdf:about="http://open-services.net/ns/auto#executesAutomationPlan">
		<rdfs:isDefinedBy rdf:resource="http://open-services.net/ns/auto#" />
		<rdfs:label>executesAutomationPlan</rdfs:label>
		<rdfs:comment>Automation Plan run by the Automation Request. It is
			likely that the target resource will be an
			oslc_auto:AutomationPlan
			but that is not necessarily the case.
		</rdfs:comment>
		<rdfs:range rdf:resource="http://open-services.net/ns/auto#AutomationRequest" />
		<rdfs:seeAlso
			rdf:resource="http://open-services.net/wiki/automation/OSLC-Automation-Specification-Version-2.0/#Resource_AutomationRequest" />
	</rdf:Property>

	<rdf:Property rdf:about="http://open-services.net/ns/auto#verdict">
		<rdfs:isDefinedBy rdf:resource="http://open-services.net/ns/auto#" />
		<rdfs:label>verdict</rdfs:label>
		<rdfs:comment>Used to indicate the verdict of the automation result
			based on values defined by the automation specification and,
			optionally, by the service provider. Most often a read-only property.
			It is expected that this will be a resource reference to a definition
			of a valid automation result verdict on the service provider.
		</rdfs:comment>
		<rdfs:range rdf:resource="http://open-services.net/ns/auto#AutomationResult" />
		<rdfs:seeAlso
			rdf:resource="http://open-services.net/wiki/automation/OSLC-Automation-Specification-Version-2.0/#Resource_AutomationResult" />
	</rdf:Property>

	<rdf:Property rdf:about="http://open-services.net/ns/auto#hasContribution">
		<rdfs:isDefinedBy rdf:resource="http://open-services.net/ns/auto#" />
		<rdfs:label>contribution</rdfs:label>
		<rdfs:comment>A result contribution associated with this automation
			result. It is recommended that the contribution be an inline resource
			which can be retrieved with the automation result. The recommended
			attributes beyond the contribution itself are dcterms:title,
			dcterms:description and dcterms:type to provide a description of the
			contribution which would be appropriate for display in a simple UI
			for an automation result.
		</rdfs:comment>
		<rdfs:range rdf:resource="http://open-services.net/ns/auto#AutomationResult" />
		<rdfs:seeAlso
			rdf:resource="http://open-services.net/wiki/automation/OSLC-Automation-Specification-Version-2.0/#Resource_AutomationResult" />
	</rdf:Property>

	<rdf:Property rdf:about="http://open-services.net/ns/auto#outputParameter">
		<rdfs:isDefinedBy rdf:resource="http://open-services.net/ns/auto#" />
		<rdfs:label>outputParameter</rdfs:label>
		<rdfs:comment>Automation Result output parameters are parameters
			associated with the automation execution which produced this Result.
			This includes the final value of all parameters used to initiate the
			execution and any additional parameters which may have been created
			during automation execution by the service provider or external
			agents. The value of a given `oslc_auto:outputParameter` MAY change
			as the execution proceeds. Point-in-time accuracy of the values of
			output parameters is not covered by this specification. Once the
			Automation Result is in a final state ( `oslc_auto:complete` or
			`oslc_auto:canceled`), the `oslc_auto:outputParameter` values MUST
			NOT change.</rdfs:comment>
		<rdfs:range rdf:resource="http://open-services.net/ns/auto#AutomationResult" />
		<rdfs:seeAlso
			rdf:resource="http://open-services.net/wiki/automation/OSLC-Automation-Specification-Version-2.0/#Resource_AutomationResult" />
	</rdf:Property>

	<rdf:Property
		rdf:about="http://open-services.net/ns/auto#producedByAutomationRequest">
		<rdfs:isDefinedBy rdf:resource="http://open-services.net/ns/auto#" />
		<rdfs:label>producedByAutomationRequest</rdfs:label>
		<rdfs:comment>Automation Request which produced the Automation Result.
			It is likely that the target resource
			will be an
			oslc_auto:AutomationResult but that is not necessarily the
			case.
		</rdfs:comment>
		<rdfs:range rdf:resource="http://open-services.net/ns/auto#AutomationResult" />
		<rdfs:seeAlso
			rdf:resource="http://open-services.net/wiki/automation/OSLC-Automation-Specification-Version-2.0/#Resource_AutomationResult" />
	</rdf:Property>

	<rdf:Property
		rdf:about="http://open-services.net/ns/auto#reportsOnAutomationPlan">
		<rdfs:isDefinedBy rdf:resource="http://open-services.net/ns/auto#" />
		<rdfs:label>reportsOnAutomationPlan</rdfs:label>
		<rdfs:comment>Automation Plan which the Automation Result reports on.
			It is likely that the target resource
			will be an
			oslc_auto:AutomationPlan but that is not necessarily the case.
		</rdfs:comment>
		<rdfs:range rdf:resource="http://open-services.net/ns/auto#AutomationResult" />
		<rdfs:seeAlso
			rdf:resource="http://open-services.net/wiki/automation/OSLC-Automation-Specification-Version-2.0/#Resource_AutomationResult" />
	</rdf:Property>

	<rdf:Description rdf:about="http://open-services.net/ns/auto#passed">
		<rdfs:isDefinedBy rdf:resource="http://open-services.net/ns/auto#" />
		<rdfs:label>passed</rdfs:label>
		<rdfs:comment>Used to indicate an automation result represents a
			successful execution.
		</rdfs:comment>
		<rdfs:seeAlso
			rdf:resource="http://open-services.net/wiki/automation/OSLC-Automation-Specification-Version-2.0/" />
	</rdf:Description>

	<rdf:Description rdf:about="http://open-services.net/ns/auto#warning">
		<rdfs:isDefinedBy rdf:resource="http://open-services.net/ns/auto#" />
		<rdfs:label>warning</rdfs:label>
		<rdfs:comment>Used to indicate an automation result represents an
			execution which encountered conditions
			which prevented successful
			execution but did not result in a failed
			execution.
		</rdfs:comment>
		<rdfs:seeAlso
			rdf:resource="http://open-services.net/wiki/automation/OSLC-Automation-Specification-Version-2.0/" />
	</rdf:Description>

	<rdf:Description rdf:about="http://open-services.net/ns/auto#fail">
		<rdfs:isDefinedBy rdf:resource="http://open-services.net/ns/auto#" />
		<rdfs:label>failed</rdfs:label>
		<rdfs:comment>Used to indicate an automation result represents a
			failed execution.
		</rdfs:comment>
		<rdfs:seeAlso
			rdf:resource="http://open-services.net/wiki/automation/OSLC-Automation-Specification-Version-2.0/" />
	</rdf:Description>

	<rdf:Description rdf:about="http://open-services.net/ns/auto#error">
		<rdfs:isDefinedBy rdf:resource="http://open-services.net/ns/auto#" />
		<rdfs:label>error</rdfs:label>
		<rdfs:comment>Used to indicate an automation result has completed but
			did not run successfully due
			to some error. This could be a timeout,
			automation coding error,
			network problem or other error
			which prevented
			the automation from running successfully to a pass,
			warning or fail
			verdict.
		</rdfs:comment>
		<rdfs:seeAlso
			rdf:resource="http://open-services.net/wiki/automation/OSLC-Automation-Specification-Version-2.0/" />
	</rdf:Description>

	<rdf:Description rdf:about="http://open-services.net/ns/auto#unavailable">
		<rdfs:isDefinedBy rdf:resource="http://open-services.net/ns/auto#" />
		<rdfs:label>unavailable</rdfs:label>
		<rdfs:comment>Used to indicate an automation result is in a state
			where a final verdict such as
			oslc:auto_pass or oslc_auto:fail is not
			yet available. Usually used when the result
			is in a
			state other than
			oslc_auto:complete.
		</rdfs:comment>
		<rdfs:seeAlso
			rdf:resource="http://open-services.net/wiki/automation/OSLC-Automation-Specification-Version-2.0/" />
	</rdf:Description>

	<rdf:Description rdf:about="http://open-services.net/ns/auto#new">
		<rdfs:isDefinedBy rdf:resource="http://open-services.net/ns/auto#" />
		<rdfs:label>new</rdfs:label>
		<rdfs:comment>Used to indicate an automation request or result has
			just been created in the service
			provider and has not yet been acted
			upon.
		</rdfs:comment>
		<rdfs:seeAlso
			rdf:resource="http://open-services.net/wiki/automation/OSLC-Automation-Specification-Version-2.0/" />
	</rdf:Description>

	<rdf:Description rdf:about="http://open-services.net/ns/auto#queued">
		<rdfs:isDefinedBy rdf:resource="http://open-services.net/ns/auto#" />
		<rdfs:label>queued</rdfs:label>
		<rdfs:comment>Primarily used to indicate an automation request or
			result is queued for additional
			actions by the service provider.
		</rdfs:comment>
		<rdfs:seeAlso
			rdf:resource="http://open-services.net/wiki/automation/OSLC-Automation-Specification-Version-2.0/" />
	</rdf:Description>

	<rdf:Description rdf:about="http://open-services.net/ns/auto#inProgress">
		<rdfs:isDefinedBy rdf:resource="http://open-services.net/ns/auto#" />
		<rdfs:label>inProgress</rdfs:label>
		<rdfs:comment>Used to indicate an automation request or result is
			active in the service provider.
		</rdfs:comment>
		<rdfs:seeAlso
			rdf:resource="http://open-services.net/wiki/automation/OSLC-Automation-Specification-Version-2.0/" />
	</rdf:Description>

	<rdf:Description rdf:about="http://open-services.net/ns/auto#canceling">
		<rdfs:isDefinedBy rdf:resource="http://open-services.net/ns/auto#" />
		<rdfs:label>canceling</rdfs:label>
		<rdfs:comment>Used to indicate the service provider is in the process
			of canceling an automation request or result.
		</rdfs:comment>
		<rdfs:seeAlso
			rdf:resource="http://open-services.net/wiki/automation/OSLC-Automation-Specification-Version-2.0/" />
	</rdf:Description>

	<rdf:Description rdf:about="http://open-services.net/ns/auto#canceled">
		<rdfs:isDefinedBy rdf:resource="http://open-services.net/ns/auto#" />
		<rdfs:label>canceled</rdfs:label>
		<rdfs:comment>Used to indicate that an automation request or result
			has been canceled.
		</rdfs:comment>
		<rdfs:seeAlso
			rdf:resource="http://open-services.net/wiki/automation/OSLC-Automation-Specification-Version-2.0/" />
	</rdf:Description>

	<rdf:Description rdf:about="http://open-services.net/ns/auto#complete">
		<rdfs:isDefinedBy rdf:resource="http://open-services.net/ns/auto#" />
		<rdfs:label>complete</rdfs:label>
		<rdfs:comment>Used to indicate that an automation request or result is
			complete.
		</rdfs:comment>
		<rdfs:seeAlso
			rdf:resource="http://open-services.net/wiki/automation/OSLC-Automation-Specification-Version-2.0/" />
	</rdf:Description>

	<!-- New terms in Automation 2.1 -->
	
	<rdfs:Class rdf:about="http://open-services.net/ns/auto#TeardownAction">
		<rdfs:isDefinedBy rdf:resource="http://open-services.net/ns/auto#" />
		<rdfs:subClassOf rdf:resource="http://open-services.net/ns/core#Action" />
		<rdfs:label>TeardownAction</rdfs:label>
		<rdfs:comment>An action that tears down a previously deployed resource. 
		It is likely that the resource was deployed using an OSLC Automation deployment plan, but this is not always the case. 
		That is, a tear-down action typically has the opposite semantics from a oslc_auto:Deploy sub-domain Automation Plan or Request, 
		even if the service provider offers no equivalents in its Automation Plan collection.</rdfs:comment>
		<rdfs:seeAlso
			rdf:resource="http://open-services.net/wiki/automation/OSLC-Automation-Specification-Version-2.1/#Teardown-action-type" />
		<rdfs:seeAlso
			rdf:resource="http://open-services.net/wiki/core/Actions-2.0/" />
	</rdfs:Class>

	<rdf:Property
		rdf:about="http://open-services.net/ns/auto#usesExecutionEnvironment">
		<rdfs:isDefinedBy rdf:resource="http://open-services.net/ns/auto#" />
		<rdfs:label>usesExecutionEnvironment</rdfs:label>
		<rdfs:comment>A resource representing the environment(s) which this Automation Plan can be executed in. 
		The execution environment resource could represent a grouping of environmental details such as operating system, database, browser, compiler, etc.
		</rdfs:comment>
		<rdfs:seeAlso
			rdf:resource="http://open-services.net/wiki/automation/OSLC-Automation-Specification-Version-2.1/#AutomationPlan-Properties" />
	</rdf:Property>

	<rdf:Description rdf:about="http://open-services.net/ns/auto#ImmediateExecution">
		<rdfs:isDefinedBy rdf:resource="http://open-services.net/ns/auto#" />
		<rdfs:label>ImmediateExecution</rdfs:label>
		<rdfs:comment>A resource that creates an Automation Request that is eligible for execution as soon as it is created, 
		as defined by the OSLC Automation specification. 
		For example, when used as an oslc:usage value on an oslc:Dialog, it indicates that it is a creation dialog for Automation Requests that are eligible for execution. 
		oslc:Dialog resources that use this as an oslc:usage value are compatible with Automation request creation dialog behaviour from OSLC Automation 2.0.
		</rdfs:comment>
		<rdfs:seeAlso
			rdf:resource="http://open-services.net/wiki/automation/OSLC-Automation-Specification-Version-2.1/" />
	</rdf:Description>

	<rdf:Description rdf:about="http://open-services.net/ns/auto#DeferredExecution">
		<rdfs:isDefinedBy rdf:resource="http://open-services.net/ns/auto#" />
		<rdfs:label>DeferredExecution</rdfs:label>
		<rdfs:comment>A resource that creates an Automation Request that is ineligible for immediate execution, 
		as defined by the OSLC Automation specification. For example, when used on as an oslc:usage value an oslc:Dialog, 
		it indicates that it is a creation dialog for Automation Requests that are not eligible for execution.
		</rdfs:comment>
		<rdfs:seeAlso
			rdf:resource="http://open-services.net/wiki/automation/OSLC-Automation-Specification-Version-2.1/" />
	</rdf:Description>
	
</rdf:RDF>